proof/crefine/RISCV64/ArchMove_C.thy
@@ -94,7 +94,7 @@ lemma atg_sp':
 (* FIXME: MOVE to EmptyFail *)
 lemma empty_fail_archThreadGet [intro!, wp, simp]:
   "empty_fail (archThreadGet f p)"
-  by (fastforce simp: archThreadGet_def)
+  by (wpsimp simp: archThreadGet_def)
 
 (* FIXME: move to ainvs? *)
 lemma sign_extend_canonical_address:
